Core/Typing.lean
@@ -37,6 +37,13 @@ abbrev TyEnv := List Ty
 -- def ValidHeadVariable (t : Term) (test : String -> Bool) : Prop :=
 --   ∃ x, Term.spine t = some x ∧ test x.fst
 
+inductive VecTyping (J : A -> B -> Prop) : Vec A m -> Vec B m -> Prop
+| nil : VecTyping J .nil .nil
+| cons :
+  J a b ->
+  VecTyping J as bs ->
+  VecTyping J (a::as) (b::bs)
+
 def Ty.HeadVariable (A : Ty) (test : String -> Bool) : Prop :=
   ∃ x sp, A.spine = some (x, sp) ∧ test x
 
@@ -90,12 +97,16 @@ inductive Kinding (G : List Global) : List Kind -> Ty -> Kind -> Prop
 
 notation:170 G:170 "&" Δ:170 " ⊢ " A:170 " : " K:170 => Kinding G Δ A K
 
-inductive SpineKinding (G : List Global) : SpineTy -> Prop where
+abbrev Ty.data? (c : DataConst) (G : List Global) (A : Ty) : Prop := A.HeadVariable (is_data c G)
+
+inductive SpineKinding (sv : SpCtorVariant) (G : List Global) : SpineTy -> Prop where
 | valid {Ks : Vec Kind m} {Ts : Vec _ n} :
   Vec.to_list Ks = Δ ->
   (∀ (i : Fin n), G&Δ ⊢ Ts[i] : ★) ->
   G&Δ ⊢ R : ★ ->
-  SpineKinding G ⟨m, Ks, n, Ts, R⟩
+  (∀ c, sv = .data c -> lookup_ctor? G c x R) ->
+  (sv = .openm -> ∀ (i : Fin n), Ts[i][τ].data? .opn G) ->
+  SpineKinding sv G ⟨m, Ks, n, Ts, R⟩
 
 -- inductive KindingPreamble (G : List Global) (Δ : List Kind) : List Ty -> Ty -> Ty -> Prop
 -- | done : KindingPreamble G Δ [] T T
@@ -104,16 +115,16 @@ inductive SpineKinding (G : List Global) : SpineTy -> Prop where
 --   KindingPreamble G Δ Ty T1[su A::+0] T2 ->
 --   KindingPreamble G Δ (A::Ty) (∀[K] T1) T2
 
-inductive PatternBinders : (m : Nat) -> Vec Ty m -> Pattern m -> List Ty -> Prop
-| zero : PatternBinders 0 ss ps []
+inductive PatternBinders (G : List Global) (Δ : List Kind) : (m : Nat) -> Vec Ty m -> Pattern m -> List Ty -> Prop
+| zero : PatternBinders G Δ 0 ss ps []
 | succ {Ts' : Vec _ nb} :
   lookup_spine_type G c = some ⟨na, Ks, nb, Ts, R⟩ ->
   (∀ (i : Fin na), G&Δ ⊢ As[i] : Ks[i]) ->
   Sequ.append_vec (Vec.map su As) +0 = τ ->
   (∀ (i : Fin nb), Ts'[i] = Ts[i][τ]) ->
   R' = R[τ] ->
-  PatternBinders n S p ℓ ->
-  PatternBinders (n + 1) (R'::S) (⟨c, na, As, nb⟩::p) ((Vec.to_list Ts') ++ ℓ)
+  PatternBinders G Δ n S p ℓ ->
+  PatternBinders G Δ (n + 1) (R'::S) (⟨c, na, As, nb⟩::p) ((Vec.to_list Ts') ++ ℓ)
 
 inductive CoercionProject (G : List Global) (Δ : List Kind) : Nat -> Ty -> Ty -> Prop where
 | fst_app :
@@ -132,26 +143,33 @@ inductive CoercionProject (G : List Global) (Δ : List Kind) : Nat -> Ty -> Ty -
 -- def Ty.ctor? (G : List Global) (ctor : String) (A : Ty) : Prop :=
 --   ∃ D sp, A.spine = some (D, sp) ∧ Global.ctor? G ctor D
 
-abbrev Ty.data? (c : DataConst) (G : List Global) (A : Ty) : Prop := A.HeadVariable (is_data c G)
+def Query (G : List Global) (c : DataConst) (qs : Vec String m) (Ts : Vec Ty m) : Prop :=
+  VecTyping (lookup_ctor? G c · ·) qs Ts
 
-inductive Query (G : List Global) : Vec String m -> Vec Ty m -> Prop where
-| nil : Query G .nil .nil
-| cons :
-  lookup_ctor? G q A ->
-  Query G qs As ->
-  Query G (q::qs) (A::As)
+-- inductive Query (G : List Global) (c : DataConst) : Vec String m -> Vec Ty m -> Prop where
+-- | nil : Query G c .nil .nil
+-- | cons :
+--   lookup_ctor? G c q A ->
+--   Query G c qs As ->
+--   Query G c (q::qs) (A::As)
 
-inductive Query.Match : Vec String m -> Pattern m -> Prop where
-| nil : Query.Match .nil .nil
-| cons :
-  Query.Match qs ps ->
-  p = ⟨q, na, As, nb⟩ ->
-  Query.Match (q::qs) (p::ps)
+def Query.Match (qs : Vec String m) (ps : Pattern m) : Prop :=
+  VecTyping (λ q p => ∃ na As nb, p = ⟨q, na, As, nb⟩) qs ps
+
+-- inductive Query.Match : Vec String m -> Pattern m -> Prop where
+-- | nil : Query.Match .nil .nil
+-- | cons :
+--   Query.Match qs ps ->
+--   p = ⟨q, na, As, nb⟩ ->
+--   Query.Match (q::qs) (p::ps)
 
 def OpenExhaustive (G : List Global) : Prop :=
-  ∀ {x na nb} {Ks : Vec _ na} {Ts : Vec _ nb} {R q},
+  ∀ {x na nb} {τ : Subst Ty} {As Ks : Vec _ na} {Ts Ts' : Vec _ nb} {Δ R q},
   lookup x G = some (.openm x ⟨na, Ks, nb, Ts, R⟩) ->
-  Query G q Ts ->
+  (∀ (i : Fin na), G&Δ ⊢ As[i] : Ks[i]) ->
+  Sequ.append_vec (Vec.map su As) +0 = τ ->
+  Vec.map (·[τ]) Ts = Ts' ->
+  Query G .opn q Ts' ->
   ∃ i b p, get_instance x i G = some ⟨nb, p, b⟩ ∧ Query.Match q p
 
 inductive Typing (G : List Global) : List Kind -> List Ty -> Term -> Ty -> Prop
@@ -171,16 +189,16 @@ inductive Typing (G : List Global) : List Kind -> List Ty -> Term -> Ty -> Prop
   (∀ (i : Fin m), G&Δ ⊢ As[i] : Ks[i]) ->
   Sequ.append_vec (Vec.map su As) +0 = τ ->
   (∀ (i : Fin n), Typing G Δ Γ (ts i) Ts[i][τ]) ->
-  (∀ c, v = .data c -> lookup_ctor? G x R) ->
-  (v = .openm -> ∀ (i : Fin n), Ts[i].data? .opn G) ->
+  (∀ c, v = .data c -> lookup_ctor? G c x R) ->
+  (v = .openm -> ∀ (i : Fin n), Ts[i][τ].data? .opn G) ->
   R' = R[τ] ->
   Typing G Δ Γ (.spctor v x As ts) R'
 | mtch {ss S : Fun.Vec _ m} {ps ts ξ : Fun.Vec _ n} :
   (∀ i, Typing G Δ Γ (ss i) (S i)) ->
   (∀ i, (S i).data? .cls G) ->
-  (∀ i, PatternBinders m S (ps i) (ξ i)) ->
+  (∀ i, PatternBinders G Δ m S (ps i) (ξ i)) ->
   (∀ i, Typing G Δ (ξ i ++ Γ) (ts i) T) ->
-  (∀ {q}, Query G q S -> ∃ i, Query.Match q (ps i)) ->
+  (∀ {q}, Query G .cls q S -> ∃ i, Query.Match q (ps i)) ->
   Typing G Δ Γ (.mtch m n ss ps ts) T
 ----------------------------------------------------------------------------------------------------
 ---- Guards
@@ -307,10 +325,35 @@ notation:170 G:170 "&" Δ:170 "," Γ:170 " ⊢ " t:170 " : " A:170 => Typing G �
 --   G&Δ ⊢ A : ★ ->
 --   ValidInstTy G x Δ (A -:> T)
 
+-- (m : Nat) × Vec Kind m × (n : Nat) × Vec Ty n × Ty
+
+inductive PatternPartTyping G Δ : String × (n : Nat) × Vec Ty n × Nat -> Ty -> Prop
+| valid :
+  lookup_spine_type G c = some ⟨na, Ks, nb, Bs, R⟩ ->
+  Sequ.append_vec (Vec.map su As) +0 = τ ->
+  (∀ i : Fin na, G&Δ ⊢ As[i] : Ks[i]) ->
+  R' = R[τ] ->
+  PatternPartTyping G Δ ⟨c, na, As, nb⟩ R'
+
+def PatternTyping (G : List Global) (Δ : List Kind) (ps : Pattern m) (Ts : Vec Ty m) : Prop :=
+  VecTyping (PatternPartTyping G Δ) ps Ts
+
+inductive ConstructorTyping G Δ Γ : Constructor -> Ty -> Prop
+| valid {ts : Vec Term nt} :
+  lookup_spine_type G c = some ⟨na, Ks, nt, Ts, R⟩ ->
+  (∀ i : Fin na, G&Δ ⊢ As[i] : Ks[i]) ->
+  Sequ.append_vec (Vec.map su As) +0 = τ ->
+  (∀ i : Fin nt, G&Δ,Γ ⊢ ts[i] : Ts[i][τ]) ->
+  R' = R[τ] ->
+  ConstructorTyping G Δ Γ ⟨c, na, As, nt, ts⟩ R'
+
+def VecConstructorTyping (G : List Global) (Δ : List Kind) (Γ : List Ty) (cs : Vec Constructor n) (Ts : Vec Ty n) : Prop :=
+  VecTyping (ConstructorTyping G Δ Γ) cs Ts
+
 inductive GlobalWf : List Global -> Global -> Prop where
 | data {G : GlobalEnv} {ctors : Fun.Vec (String × SpineTy) n} :
   (∀ i y T, ctors i = (y, T) ->
-    SpineKinding (.data 0 x K .nil::G) T
+    SpineKinding (.data .cls) (.data 0 x K .nil::G) T
     ∧ x ≠ y
     ∧ lookup y G = none) ->
   (∀ i j, (ctors i).1 ≠ (ctors j).1) ->
@@ -320,7 +363,7 @@ inductive GlobalWf : List Global -> Global -> Prop where
   lookup x G = none ->
   GlobalWf G (.odata x K)
 | openm {Γ : Vec Ty n} :
-  SpineKinding G T ->
+  SpineKinding .openm G T ->
   lookup x G = none ->
   GlobalWf G (.openm x T)
 | defn :
@@ -335,7 +378,7 @@ inductive GlobalWf : List Global -> Global -> Prop where
   G&Δ,Γ ⊢ t : R ->
   GlobalWf G (.inst x p t)
 | instty :
-  SpineKinding G T ->
+  SpineKinding (.data .opn) G T ->
   lookup x G = none ->
   GlobalWf G (.octor x T)
 
